ERT/Stlc/DeBruijn/Semantics.lean
@@ -13,6 +13,15 @@ def AtT.den {α} [τ: SemanticConst α] {Γ: Ctx τ.Base} {n: ℕ} {A: _}
   | AtT.head _ _, (x, _G) => x
   | AtT.tail _ v, (_x, G) => AtT.den v G
 
+theorem AtT.den_head {α} [τ: SemanticConst α] {Γ: Ctx τ.Base} {A x G}
+  : (AtT.head A Γ).den (x, G) = x
+  := rfl
+
+def AtT.den_tail {α} [τ: SemanticConst α] {Γ: Ctx τ.Base}
+  {A: Ty τ.Base} {n} {v: AtT Γ n A} {x} {G: Γ.den}
+  : (AtT.tail A v).den (x, G) = v.den G
+  := rfl
+
 def At.den_eq_app {α} [τ: SemanticConst α] {Γ: Ctx τ.Base} {n: ℕ} {A: _}
   : (v: At Γ n A) -> (G: Γ.den) -> v.den G = v.toAtT.den G
   | At.head _ _, (_, _) => rfl
@@ -20,6 +29,9 @@ def At.den_eq_app {α} [τ: SemanticConst α] {Γ: Ctx τ.Base} {n: ℕ} {A: _}
 
 def At.den_eq {α} [τ: SemanticConst α] {Γ: Ctx τ.Base} {n: ℕ} {A: _} (v: At Γ n A)
   : v.den = v.toAtT.den := by funext _; rw [At.den_eq_app]
+
+def AtT.den_eq {α} [τ: SemanticConst α] {Γ: Ctx τ.Base} {n: ℕ} {A: _} (v: AtT Γ n A)
+  : v.den = v.toAt.den := by rw [At.den_eq]; apply congrArg; apply Subsingleton.allEq
 
 def WkListT.den {α} [τ: SemanticConst α] {Γ Δ: Ctx τ.Base}
   : WkListT ρ Γ Δ -> Γ.den -> Δ.den
@@ -30,6 +42,49 @@ def WkListT.den {α} [τ: SemanticConst α] {Γ Δ: Ctx τ.Base}
 def WkList.den {α} [τ: SemanticConst α] {Γ Δ: Ctx τ.Base} (R: WkList ρ Γ Δ)
   : Γ.den -> Δ.den
   := R.toWkListT.den
+
+def WkList.den_eq_app {α} [τ: SemanticConst α] {Γ Δ: Ctx τ.Base}
+  (R: WkList ρ Γ Δ) (G: Γ.den): R.den G = R.toWkListT.den G
+  := rfl
+
+def WkList.den_eq {α} [τ: SemanticConst α] {Γ Δ: Ctx τ.Base}
+  (R: WkList ρ Γ Δ): R.den = R.toWkListT.den
+  := rfl
+
+def AtT.den_wk_t_app {α} [τ: SemanticConst α] {Γ Δ: Ctx τ.Base} {n: ℕ} {A: _}
+  : (R: WkListT ρ Γ Δ) -> (v: AtT Δ n A)
+    -> (G: Γ.den) -> (v.wk_t R).den G = v.den (R.den G)
+  | WkListT.step _ R, v, (x, G) => by rw [WkListT.den, wk_t, den, den_wk_t_app R v G]
+  | WkListT.lift _ R, AtT.head _ _, (x, G) => by rw [WkListT.den, den, wk_t, den]
+  | WkListT.lift _ R, AtT.tail _ v, (x, G) => by
+    rw [WkListT.den, den, wk_t, den, den_wk_t_app R v G]
+
+def AtT.den_wk_t {α} [τ: SemanticConst α] {Γ Δ: Ctx τ.Base} {n: ℕ} {A: _}
+  (R: WkListT ρ Γ Δ) (v: AtT Δ n A): (v.wk_t R).den = v.den ∘ R.den
+  := by funext _; apply den_wk_t_app
+
+def At.den_wk {α} [τ: SemanticConst α] {Γ Δ: Ctx τ.Base} {n: ℕ} {A: _}
+  (R: WkList ρ Γ Δ) (v: At Δ n A): (v.wk R).den = v.den ∘ R.den := by
+  rw [At.den_eq, At.den_eq, WkList.den_eq, <-AtT.den_wk_t]
+  apply congrArg
+  apply Subsingleton.allEq
+
+def At.den_wk_app {α} [τ: SemanticConst α] {Γ Δ: Ctx τ.Base} {n: ℕ} {A: _}
+  (R: WkList ρ Γ Δ) (v: At Δ n A) (G: Γ.den): (v.wk R).den G = v.den (R.den G) :=
+  congrFun (v.den_wk R) _
+
+def At.den_wk_t {α} [τ: SemanticConst α] {Γ Δ: Ctx τ.Base} {n: ℕ} {A: _}
+  (R: WkListT ρ Γ Δ) (v: At Δ n A): (v.wk R.toWkList).den = v.den ∘ R.den := by
+  rw [den_wk]
+  apply congrArg
+  rw [WkList.den_eq R.toWkList]
+  apply congrArg
+  apply Subsingleton.allEq
+
+def At.den_wk_t_app {α} [τ: SemanticConst α] {Γ Δ: Ctx τ.Base} {n: ℕ} {A: _}
+  (R: WkListT ρ Γ Δ) (v: At Δ n A) (G: Γ.den)
+  : (v.wk R.toWkList).den G = v.den (R.den G) :=
+  congrFun (v.den_wk_t R) _
 
 namespace Stlc.DeBruijn
 
@@ -64,3 +119,60 @@ def HasTy.den {α} [τ: SemanticConst α] {Γ} {a: Term α} {A}
     pure (Sum.inr t)
   | HasTy.cnst c, G => τ.cnstDen c
   | HasTy.abort _, _ => τ.abort _
+
+def HasTy.den_wk_t_app {α} [τ: SemanticConst α] {ρ} {Γ Δ: Ctx τ.Base} {a: Term α} {A}
+  (R: WkListT ρ Γ Δ): (H: HasTy Δ a A) ->
+    (G: Γ.den) -> (H.wk R.toWkList).den G = H.den (R.den G)
+  | HasTy.var v, G => v.den_wk_t_app R G
+  | HasTy.app s t, G => by
+    rw [HasTy.den, <-HasTy.den_wk_t_app R s G, <-HasTy.den_wk_t_app R t G]
+    rfl
+  | HasTy.lam t, G => by
+    rw [HasTy.den, wk, HasTy.den]
+    apply congrArg
+    funext x
+    rw [HasTy.den_wk_t_app, WkListT.den]
+  | HasTy.pair s t, G => by
+    rw [HasTy.den, <-HasTy.den_wk_t_app R s G, <-HasTy.den_wk_t_app R t G]
+    rfl
+  | HasTy.let1 s t, G => by
+    rw [HasTy.den, wk, HasTy.den,
+      <-HasTy.den_wk_t_app R s G]
+    apply congrArg
+    funext s
+    rw [HasTy.den_wk_t_app _ t _, WkListT.den]
+  | HasTy.let2 s t, G => by
+    rw [HasTy.den, wk, HasTy.den,
+      <-HasTy.den_wk_t_app R s G]
+    apply congrArg
+    funext ⟨x, y⟩
+    simp only []
+    rw [HasTy.den_wk_t_app _ t _, WkListT.den, WkListT.den]
+  | HasTy.case e l r, G => by
+    rw [HasTy.den, <-HasTy.den_wk_t_app R e G, wk, HasTy.den]
+    apply congrArg
+    funext e
+    split
+    . rw [HasTy.den_wk_t_app _ l _, WkListT.den]
+    . rw [HasTy.den_wk_t_app _ r _, WkListT.den]
+  | HasTy.inl t, G => by
+    rw [HasTy.den, <-HasTy.den_wk_t_app R t G]
+    rfl
+  | HasTy.inr t, G => by
+    rw [HasTy.den, <-HasTy.den_wk_t_app R t G]
+    rfl
+  | HasTy.cnst c, G => rfl
+  | HasTy.abort _, _ => rfl
+
+def HasTy.den_wk_t {α} [τ: SemanticConst α] {ρ} {Γ Δ: Ctx τ.Base} {a: Term α} {A}
+  (R: WkListT ρ Γ Δ) (H: HasTy Δ a A): (H.wk R.toWkList).den = H.den ∘ R.den := by
+  funext G; rw [den_wk_t_app]; rfl
+
+def HasTy.den_wk_app {α} [τ: SemanticConst α] {ρ} {Γ Δ: Ctx τ.Base} {a: Term α} {A}
+  (R: WkList ρ Γ Δ) (H: HasTy Δ a A) (G: Γ.den): (H.wk R).den G = H.den (R.den G) := by
+  rw [den_wk_t_app R.toWkListT]
+  rfl
+
+def HasTy.den_wk {α} [τ: SemanticConst α] {ρ} {Γ Δ: Ctx τ.Base} {a: Term α} {A}
+  (R: WkList ρ Γ Δ) (H: HasTy Δ a A): (H.wk R).den = H.den ∘ R.den := by
+   funext G; rw [den_wk_app]; rfl
